vera/EnvStack.v
@@ -4,58 +4,63 @@ Import ListNotations.
 
 From Equations Require Import Equations.
 
-Definition t A := list (NameMap.t A).
+Module M(M: FMapInterface.WS).
+  Module Extras := MapExtras(M).
+  Module Facts := FMapFacts.Facts(M).
 
-Definition empty (A : Type) : t A := [NameMap.empty A].
+  Definition t A := list (M.t A).
 
-Equations lookup {A} : NameMap.key -> t A -> option A :=
-  lookup n [] := None;
-  lookup n (m :: ms) :=
-    match NameMap.find n m with
-    | None => lookup n ms
-    | Some x => Some x
-    end
-.
+  Definition empty (A : Type) : t A := [M.empty A].
 
-Equations add {A} : NameMap.key -> A -> t A -> t A :=
-  add n v [] := [];
-  add n v (m :: ms) := NameMap.add n v m :: ms
-.
+  Equations lookup {A} : M.key -> t A -> option A :=
+    lookup n [] := None;
+    lookup n (m :: ms) :=
+      match M.find n m with
+      | None => lookup n ms
+      | Some x => Some x
+      end
+  .
 
-Definition push {A} (env : t A) : t A :=
-  NameMap.empty A :: env
-.
+  Equations add {A} : M.key -> A -> t A -> t A :=
+    add n v [] := [];
+    add n v (m :: ms) := M.add n v m :: ms
+  .
 
-Equations pop {A} : t A -> option (NameMap.t A) * t A :=
-  pop (m :: ms) := (Some m, ms);
-  pop [] := (None, [])
-.
+  Definition push {A} (env : t A) : t A :=
+    M.empty A :: env
+  .
 
-Equations flatten {A} : t A -> NameMap.t A :=
-  flatten [] := NameMap.empty A;
-  flatten (m::ms) := NameMap.combine m (flatten ms)
-.
+  Equations pop {A} : t A -> option (M.t A) * t A :=
+    pop (m :: ms) := (Some m, ms);
+    pop [] := (None, [])
+  .
 
-Section Correct.
-  Lemma lookup_push :
-    forall A (E : t A) k,
-    lookup k (push E) = lookup k E.
-  Proof.
-    intros.
-    unfold push.
-    simp lookup.
-    rewrite StrMap.empty_o.
-    reflexivity.
-  Qed.
+  Equations flatten {A} : t A -> M.t A :=
+    flatten [] := M.empty A;
+    flatten (m::ms) := Extras.combine m (flatten ms)
+  .
 
-  Lemma lookup_empty :
-    forall A (E : t A) k,
-    lookup k (empty A) = None.
-  Proof.
-    intros.
-    unfold empty.
-    simp lookup.
-    rewrite StrMap.empty_o.
-    reflexivity.
-  Qed.
-End Correct.
+  Section Correct.
+    Lemma lookup_push :
+      forall A (E : t A) k,
+        lookup k (push E) = lookup k E.
+    Proof.
+      intros.
+      unfold push.
+      simp lookup.
+      rewrite Facts.empty_o.
+      reflexivity.
+    Qed.
+
+    Lemma lookup_empty :
+      forall A (E : t A) k,
+        lookup k (empty A) = None.
+    Proof.
+      intros.
+      unfold empty.
+      simp lookup.
+      rewrite Facts.empty_o.
+      reflexivity.
+    Qed.
+  End Correct.
+End M.
