vera/Verilog.v
@@ -3,6 +3,7 @@ From Coq Require Import ZArith.
 From Coq Require Import BinNums.
 
 From nbits Require Import NBits.
+From mathcomp Require Import seq.
 
 From vera Require Import Common.
 
@@ -128,6 +129,14 @@ Module TypedVerilog.
   | IntegerLiteral : bits -> expression
   | NamedExpression : vtype -> string -> expression
   .
+
+  Equations expr_type : TypedVerilog.expression -> Verilog.vtype :=
+    expr_type (TypedVerilog.BinaryOp t _ _ _) := t;
+    expr_type (TypedVerilog.BitSelect _ _) := 0;
+    expr_type (TypedVerilog.Conditional _ tBranch fBranch) := expr_type tBranch; (**  TODO: need to check fBranch? *)
+    expr_type (TypedVerilog.Conversion _ t _) := t;
+    expr_type (TypedVerilog.IntegerLiteral v) := size v;
+    expr_type (TypedVerilog.NamedExpression t _) := t.
 
   Inductive Statement :=
   | Block (body : list Statement)
