vera/VerilogCanonicalize.v
@@ -1,0 +1,254 @@
+From Coq Require Import List.
+From Coq Require Import Program.
+From Coq Require Import String.
+
+From Equations Require Import Equations.
+From ExtLib Require Import Data.List.
+From ExtLib Require Import Data.Monads.EitherMonad.
+From ExtLib Require Import Data.Monads.StateMonad.
+From ExtLib Require Import Data.String.
+From ExtLib Require Import Structures.Applicative.
+From ExtLib Require Import Structures.Functor.
+From ExtLib Require Import Structures.MonadExc.
+From ExtLib Require Import Structures.MonadState.
+From ExtLib Require Import Structures.Monads.
+From ExtLib Require Import Structures.Traversable.
+From ExtLib Require Import Programming.Show.
+From nbits Require Import NBits.
+
+From vera Require Import Verilog.
+From vera Require Import Common.
+From vera Require EnvStack.
+
+Import ListNotations.
+Import CommonNotations.
+Import MonadNotation.
+Import FunctorNotation.
+Local Open Scope monad_scope.
+Local Open Scope bits_scope.
+
+Module StrEnvStack := EnvStack.M(StrMap).
+
+Record state :=
+  TransfState
+    { initialStatements : list TypedVerilog.Statement
+    ; substitutionsBlocking : StrEnvStack.t TypedVerilog.expression
+    ; substitutionsNonblocking : StrEnvStack.t TypedVerilog.expression
+    }.
+
+Definition transf : Type -> Type := stateT state (sum string).
+
+Global Instance Monad_transf : Monad transf := Monad_stateT state (Monad_either string).
+
+Definition run_transf_test {T} (a : transf T) :=
+      runStateT
+        a
+        {| initialStatements := []
+        ; substitutionsBlocking := StrEnvStack.empty _
+        ; substitutionsNonblocking := StrEnvStack.empty _
+        |}.
+
+Definition run_transf {T} (a : transf T) :=
+      runStateT
+        a
+        {| initialStatements := []
+        ; substitutionsBlocking := StrEnvStack.empty _
+        ; substitutionsNonblocking := StrEnvStack.empty _
+        |}.
+
+Definition set_substitution_blocking (lhs : string) (rhs : TypedVerilog.expression) : transf () :=
+  modify (fun s =>
+            {| initialStatements := initialStatements s
+            ; substitutionsBlocking := StrEnvStack.add lhs rhs (substitutionsBlocking s)
+            ; substitutionsNonblocking := substitutionsNonblocking s
+            |}) ;;
+  ret ()
+.
+
+Definition set_substitution_nonblocking (lhs : string) (rhs : TypedVerilog.expression) : transf () :=
+  modify (fun s =>
+            {| initialStatements := initialStatements s
+            ; substitutionsBlocking := substitutionsBlocking s
+            ; substitutionsNonblocking := StrEnvStack.add lhs rhs (substitutionsNonblocking s)
+            |}) ;;
+  ret ()
+.
+
+Definition push_block : transf () :=
+  modify (fun s =>
+            {| initialStatements := initialStatements s
+            ; substitutionsBlocking := StrEnvStack.push (substitutionsBlocking s)
+            ; substitutionsNonblocking := StrEnvStack.push (substitutionsNonblocking s)
+            |}) ;;
+  ret ()
+.
+
+Definition pop_block : transf (StrMap.t TypedVerilog.expression * StrMap.t TypedVerilog.expression) :=
+  s <- get ;;
+  let (mBlockingEnv, substitutionsBlocking') := StrEnvStack.pop (substitutionsBlocking s) in
+  let (mNonblockingEnv, substitutionsNonblocking') := StrEnvStack.pop (substitutionsNonblocking s) in
+  match mBlockingEnv, mNonblockingEnv with
+  | Some benv, Some nbenv =>
+      modify (fun s =>
+                {| initialStatements := initialStatements s
+                ; substitutionsBlocking := substitutionsBlocking'
+                ; substitutionsNonblocking := substitutionsNonblocking'
+                |}) ;;
+      ret (benv, nbenv)
+  | _, _ =>
+      raise "pop_block with an empty stack"%string
+  end
+.
+
+Definition add_initial_statements (statements : list TypedVerilog.Statement) : transf () :=
+  modify (fun s =>
+            {| initialStatements := initialStatements s ++ statements
+            ; substitutionsBlocking := StrEnvStack.push (substitutionsBlocking s)
+            ; substitutionsNonblocking := StrEnvStack.push (substitutionsNonblocking s)
+            |}) ;;
+  ret ()
+.
+
+
+Definition transfer_scoped {A} (f : transf A) : transf (A * (StrMap.t TypedVerilog.expression * StrMap.t TypedVerilog.expression)) :=
+  push_block ;;
+  result <- f ;;
+  assigns <- pop_block ;;
+  ret (result, assigns)
+.
+
+Equations transfer_expression : TypedVerilog.expression -> transf TypedVerilog.expression :=
+| TypedVerilog.NamedExpression t n =>
+    st <- get ;;
+    match StrEnvStack.lookup n (substitutionsBlocking st) with
+    | Some e => ret e
+    | None => ret (TypedVerilog.NamedExpression t n)
+    end
+| e => ret e
+.
+
+Definition decide_or_fail {P : Prop} (dec : { P } + { ~ P }) (msg : string) : transf P :=
+  match dec with
+  | left prf => ret prf
+  | right _ => raise msg
+  end
+.
+
+Program Definition merge_if
+  (setter : string -> TypedVerilog.expression -> transf ())
+  (cond : TypedVerilog.expression)
+  (defaults substitutionsTrue substitutionsFalse : StrMap.t TypedVerilog.expression)
+  : transf () :=
+  let substitutions_combined :=
+    StrMap.elements (StrMap.union_both defaults (StrMap.union_both substitutionsTrue substitutionsFalse)) in
+
+  mapT (
+      fun  (it : (string * (option TypedVerilog.expression * option (option TypedVerilog.expression * option TypedVerilog.expression)))) =>
+        st <- get ;;
+        let '(n, (default, branches )) := it in
+        match branches with
+        | Some (trueBranch, falseBranch) =>
+            match trueBranch, falseBranch with
+            | Some t, Some f =>
+                width_ok <- decide_or_fail
+                             (eq_dec (TypedVerilog.expr_type t) (TypedVerilog.expr_type f))
+                             "Incompatible widths in conditional";;
+                setter n (TypedVerilog.Conditional cond t f)
+            | Some t, None =>
+                let def := opt_or_else default (TypedVerilog.NamedExpression (TypedVerilog.expr_type t) n) in
+                setter n (TypedVerilog.Conditional cond t def)
+            | None, Some f =>
+                let def := opt_or_else default (TypedVerilog.NamedExpression (TypedVerilog.expr_type f) n) in
+                setter n (TypedVerilog.Conditional cond def f)
+            | None, None => raise "Invalid state in merge_if"%string
+            end
+        | None => ret ()
+        end
+    ) substitutions_combined ;;
+  ret ()
+.
+
+(*
+  Translated from the following
+https://github.com/CakeML/hardware/blob/8264e60f0f9d503c9d971991cf181012276f0c9b/compiler/RTLCompilerScript.sml#L233-L295
+*)
+Equations transfer_statement : TypedVerilog.Statement -> transf () :=
+| TypedVerilog.Block body =>
+    mapT transfer_statement body ;;
+    ret ()
+| TypedVerilog.NonBlockingAssign (TypedVerilog.NamedExpression t__lhs name__lhs) rhs =>
+    input__rhs <- transfer_expression rhs ;;
+    set_substitution_nonblocking name__lhs input__rhs
+| TypedVerilog.NonBlockingAssign lhs rhs =>
+    raise "Invalid lhs for non-blocking assignment"%string
+| TypedVerilog.BlockingAssign (TypedVerilog.NamedExpression t__lhs name__lhs) rhs =>
+    input__rhs <- transfer_expression rhs ;;
+    set_substitution_blocking name__lhs input__rhs
+| TypedVerilog.BlockingAssign lhs rhs =>
+    raise "Invalid lhs for blocking assignment"%string
+| TypedVerilog.If condition trueBranch falseBranch =>
+    st <- get ;;
+    let defaults := StrEnvStack.flatten (substitutionsBlocking st) in
+    condInput <- transfer_expression condition ;;
+    '(_, (blockingTrue, nonblockingTrue)) <- transfer_scoped (transfer_statement trueBranch) ;;
+    '(_, (blockingFalse, nonblockingFalse)) <- transfer_scoped (transfer_statement falseBranch) ;;
+    merge_if set_substitution_blocking condInput defaults blockingTrue blockingFalse ;;
+    merge_if set_substitution_nonblocking condInput defaults nonblockingTrue nonblockingFalse ;;
+    ret ()
+.
+
+Equations canonicalize_module_item : TypedVerilog.module_item -> transf () :=
+| TypedVerilog.AlwaysFF body =>
+    transfer_statement body ;;
+    ret ()
+| TypedVerilog.AlwaysComb body =>
+    transfer_statement body ;;
+    ret ()
+| TypedVerilog.Initial (TypedVerilog.Block stmts) =>
+    add_initial_statements stmts
+| TypedVerilog.Initial stmt =>
+    add_initial_statements [stmt]
+.
+
+Definition substitutions_to_assignments :
+  list (string * TypedVerilog.expression) -> list TypedVerilog.Statement :=
+  map (fun '(lhs, rhs) =>
+         TypedVerilog.NonBlockingAssign
+           (* TODO: Keep the original type, rather than getting it from rhs *)
+           (TypedVerilog.NamedExpression (TypedVerilog.expr_type rhs) lhs)
+           rhs).
+
+Definition canonicalize_module (vmodule : TypedVerilog.vmodule) : transf TypedVerilog.vmodule :=
+  mapT canonicalize_module_item (TypedVerilog.modBody vmodule) ;;
+  finalState <- get ;;
+
+  let subs :=
+    StrMap.elements
+      (StrMap.combine
+         (StrEnvStack.flatten (substitutionsNonblocking finalState))
+         (StrEnvStack.flatten (substitutionsBlocking finalState))) in
+  let always_body := substitutions_to_assignments subs in
+  let initial_body := initialStatements finalState in
+  let body := [
+      TypedVerilog.Initial (TypedVerilog.Block initial_body);
+      TypedVerilog.AlwaysFF (TypedVerilog.Block always_body)
+    ] in
+  ret
+    {|
+      TypedVerilog.modName := TypedVerilog.modName vmodule;
+      TypedVerilog.modPorts := TypedVerilog.modPorts vmodule;
+      TypedVerilog.modVariables := TypedVerilog.modVariables vmodule;
+      TypedVerilog.modBody := body
+    |}
+.
+
+Definition canonicalize_verilog
+  (vmodule : TypedVerilog.vmodule)
+  : sum string TypedVerilog.vmodule :=
+  evalStateT
+    (canonicalize_module vmodule)
+    {| initialStatements := []
+    ; substitutionsBlocking := StrEnvStack.empty _
+    ; substitutionsNonblocking := StrEnvStack.empty _
+    |}
+.
