vera/VerilogEquivalence.v
@@ -1,10 +1,9 @@
-Require Import Verilog.
-Require Import Netlist.
-Require Import VerilogToNetlist.
-Require Import NetlistToSMT.
-Require Import SMT.
-Require Import Common.
-Require VerilogTypecheck.
+From vera Require Import Verilog.
+From vera Require Import SMT.
+From vera Require Import Common.
+From vera Require VerilogTypecheck.
+From vera Require VerilogCanonicalize.
+From vera Require VerilogToSMT.
 
 From ExtLib Require Import Structures.Monads.
 From ExtLib Require Import Data.Monads.EitherMonad.
@@ -16,15 +15,15 @@ Require Import List.
 Import ListNotations.
 Import EqNotations.
 
-Definition mk_equivalence_formulas (smtnl1 smtnl2 : SMT.smt_netlist name) : sum string (list (SMT.formula name)) :=
+Definition mk_equivalence_formulas (smtnl1 smtnl2 : SMT.smt_netlist string) : sum string (list (SMT.formula string)) :=
   let inputs1 := filter (fun '(_, dir) => is_port_in dir) (SMT.smtnlPorts smtnl1) in
   let inputs2 := filter (fun '(_, dir) => is_port_in dir) (SMT.smtnlPorts smtnl2) in
   let outputs1 := filter (fun '(_, dir) => is_port_out dir) (SMT.smtnlPorts smtnl1) in
   let outputs2 := filter (fun '(_, dir) => is_port_out dir) (SMT.smtnlPorts smtnl2) in
   if negb (length inputs1 =? length inputs2) then inl "Input counts do not match"%string
   else if negb (length outputs1 =? length outputs2) then inl "Output counts do not match"%string
-       else let input_pairs: list ((name * port_direction) * (name * port_direction)) := combine inputs1 inputs2 in
-            let output_pairs: list ((name * port_direction) * (name * port_direction)) := combine outputs1 outputs2 in
+       else let input_pairs: list ((string * port_direction) * (string * port_direction)) := combine inputs1 inputs2 in
+            let output_pairs: list ((string * port_direction) * (string * port_direction)) := combine outputs1 outputs2 in
             let inputs_same :=
               map
                 (fun '((in1, _), (in2, _)) =>
@@ -37,19 +36,19 @@ Definition mk_equivalence_formulas (smtnl1 smtnl2 : SMT.smt_netlist name) : sum 
             inr (inputs_same ++ outputs_different)
 .
 
-Definition equivalence_query (verilog1 verilog2 : Verilog.vmodule) : sum string (list (SMT.formula name)) :=
+Definition equivalence_query
+  (verilog1 verilog2 : Verilog.vmodule)
+  : sum string (list (SMT.formula string)) :=
+
   typed_verilog1 <- VerilogTypecheck.tc_vmodule verilog1 ;;
   typed_verilog2 <- VerilogTypecheck.tc_vmodule verilog2 ;;
-  netlist_result1 <- verilog_to_netlist 1%positive typed_verilog1  ;;
-  let netlist1 := fst netlist_result1 in
-  let final_state := snd netlist_result1 in
-  netlist_result2 <- verilog_to_netlist (nextName final_state) typed_verilog2 ;;
-  let netlist2 := fst netlist_result2 in
-  let smt_netlist1 := netlist_to_smt netlist1 in
-  let smt_netlist2 := netlist_to_smt netlist2 in
-  let formulas1 := (SMT.smtnlFormulas smt_netlist1) in
-  let formulas2 := (SMT.smtnlFormulas smt_netlist2) in
+  canonical_verilog1 <- VerilogCanonicalize.canonicalize_verilog typed_verilog1 ;;
+  canonical_verilog2 <- VerilogCanonicalize.canonicalize_verilog typed_verilog2 ;;
+  smt_netlist1 <- VerilogToSMT.verilog_to_smt canonical_verilog1 ;;
+  smt_netlist2 <- VerilogToSMT.verilog_to_smt canonical_verilog2 ;;
+  let formulas1 := SMT.smtnlFormulas smt_netlist1 in
+  let formulas2 := SMT.smtnlFormulas smt_netlist2 in
   equivalence_formulas <- mk_equivalence_formulas smt_netlist1 smt_netlist2 ;;
   (** Add equivalence queries *)
-  ret (formulas1 ++ formulas2 ++ equivalence_formulas)
+  ret formulas1 (* (formulas1 ++ formulas2 ++ equivalence_formulas) *)
 .
