vera/VerilogToSMT.v
@@ -1,0 +1,87 @@
+From Coq Require Import BinIntDef.
+From Coq Require Import BinNums.
+From Coq Require Import FSets.
+From Coq Require Import List.
+From Coq Require Import Program.
+From Coq Require Import Psatz.
+From Coq Require Import String.
+From Coq Require Import ZArith.
+
+From Equations Require Import Equations.
+From ExtLib Require Import Data.List.
+From ExtLib Require Import Data.Monads.EitherMonad.
+From ExtLib Require Import Data.Monads.StateMonad.
+From ExtLib Require Import Data.String.
+From ExtLib Require Import Structures.Applicative.
+From ExtLib Require Import Structures.Functor.
+From ExtLib Require Import Structures.MonadExc.
+From ExtLib Require Import Structures.MonadState.
+From ExtLib Require Import Structures.Monads.
+From ExtLib Require Import Structures.Monoid.
+From ExtLib Require Import Structures.Traversable.
+From ExtLib Require Import Programming.Show.
+From nbits Require Import NBits.
+
+From vera Require Import Verilog.
+From vera Require Import SMT.
+From vera Require Import Common.
+From vera Require EnvStack.
+
+Import ListNotations.
+Import CommonNotations.
+Import MonadNotation.
+Import FunctorNotation.
+Local Open Scope monad_scope.
+Local Open Scope bits_scope.
+
+Definition transf := sum string.
+
+Definition transfer_name (n : string) : transf string := raise "not implemented"%string.
+
+Equations expr_to_smt : TypedVerilog.expression -> transf (SMT.qfbv string) :=
+  expr_to_smt (TypedVerilog.BinaryOp _ Verilog.BinaryPlus lhs rhs) :=
+    lhs__smt <- expr_to_smt lhs ;;
+    rhs__smt <- expr_to_smt rhs ;;
+    ret (SMT.BVAdd lhs__smt rhs__smt);
+  expr_to_smt (TypedVerilog.BinaryOp _ Verilog.BinaryMinus lhs rhs) :=
+    lhs__smt <- expr_to_smt lhs ;;
+    rhs__smt <- expr_to_smt rhs ;;
+    ret (SMT.BVAdd lhs__smt (SMT.BVNeg rhs__smt));
+  expr_to_smt (TypedVerilog.BinaryOp _ Verilog.BinaryStar lhs rhs) :=
+    lhs__smt <- expr_to_smt lhs ;;
+    rhs__smt <- expr_to_smt rhs ;;
+    ret (SMT.BVMul lhs__smt rhs__smt);
+  expr_to_smt (TypedVerilog.BinaryOp _ Verilog.BinaryShiftLeft lhs rhs) :=
+    lhs__smt <- expr_to_smt lhs ;;
+    rhs__smt <- expr_to_smt rhs ;;
+    ret (SMT.BVShl lhs__smt rhs__smt);
+  expr_to_smt (TypedVerilog.BinaryOp _ Verilog.BinaryShiftLeftArithmetic lhs rhs) :=
+    lhs__smt <- expr_to_smt lhs ;;
+    rhs__smt <- expr_to_smt rhs ;;
+    ret (SMT.BVShl lhs__smt rhs__smt);
+  expr_to_smt (TypedVerilog.BinaryOp _ Verilog.BinaryShiftRight lhs rhs) :=
+    lhs__smt <- expr_to_smt lhs ;;
+    rhs__smt <- expr_to_smt rhs ;;
+    ret (SMT.BVLShr lhs__smt rhs__smt);
+  expr_to_smt (TypedVerilog.BinaryOp _ _ _ _) :=
+    raise "Unsupported operator in SMT"%string;
+  expr_to_smt (TypedVerilog.Conditional cond ifT ifF) :=
+    cond__smt <- expr_to_smt cond ;;
+    ifT__smt <- expr_to_smt ifT ;;
+    ifF__smt <- expr_to_smt ifF ;;
+    ret (SMT.CoreITE cond__smt ifT__smt ifF__smt);
+  expr_to_smt (TypedVerilog.BitSelect vec idx) :=
+    vec__smt <- expr_to_smt vec ;;
+    idx__smt <- expr_to_smt idx ;;
+    ret (SMT.BVExtract 0 0 (SMT.BVLShr vec__smt idx__smt));
+  expr_to_smt (TypedVerilog.Conversion from to expr) :=
+    _;
+  expr_to_smt (TypedVerilog.IntegerLiteral val) :=
+    ret (SMT.BVLit val);
+  expr_to_smt (TypedVerilog.NamedExpression t n) :=
+    n__smt <- transfer_name n ;;
+    ret (SMT.BVVar n__smt).
+
+Definition verilog_to_smt
+  (vmodule : TypedVerilog.vmodule)
+  : sum string (SMT.smt_netlist string) := raise "not_implemented"%string.
